AVM/Scope/Label.lean
@@ -1,12 +1,19 @@
 import AVM.Ecosystem.Label
 
+import Lean
+open Lean
+
 namespace AVM.Scope
 
 structure Label where
   EcosystemId : Type
+  EcosystemIdEnum : FinEnum EcosystemId
   ecosystem : EcosystemId → Ecosystem.Label
 
 namespace Label
+
+-- TODO rename/remove
+abbrev fin (s : Label) : Fin s.EcosystemIdEnum.card → s.EcosystemId := s.EcosystemIdEnum.equiv.invFun
 
 abbrev EcosystemId.label {lab : Label} (e : lab.EcosystemId) : Ecosystem.Label :=
   lab.ecosystem e
@@ -21,4 +28,10 @@ end Scope.Label
 
 abbrev Ecosystem.Label.toScope (lab : Ecosystem.Label) : Scope.Label where
   EcosystemId := Unit
+  EcosystemIdEnum := {
+    card := 1
+    equiv := {
+      toFun := fun _ => 0
+      invFun := fun _ => .unit
+      right_inv := by grind}}
   ecosystem := fun .unit => lab
